playing around with proofs

compiler/backend/proofs/bvi_tmcProofScript.sml
@@ -3,9 +3,28 @@
 *)
 Theory bvi_tmcProof
 Ancestors
-  bvi_tmc (* bviProps bviSem *)
+  bvi_tmc bviProps bviSem
 Libs
   preamble
+
+val s = mk_var("s",
+  type_of ``bviSem$evaluate`` |> strip_fun |> snd |> dest_prod |> snd
+  |> type_subst [alpha|->``:num#'c``,beta|->``:'ffi``]);
+
+(* Copied - TODO *)
+Definition env_rel_def:
+  env_rel (*ty opt acc*) env1 env2 <=>
+    isPREFIX env1 env2 (* ∧
+    (opt ⇒
+      LENGTH env1 = acc ∧
+      LENGTH env2 > acc ∧
+      case ty of
+        Int => ?k. EL acc env2 = Number k
+      | List => ?ys. v_to_list (EL acc env2) = SOME ys
+      | Any => F) *)
+End
+
+Overload in_ns_2[local] = ``λn. n MOD bvl_to_bvi_namespaces = 2``
 
 Definition code_rel_def:
   code_rel c1 c2 ⇔
@@ -21,38 +40,146 @@ Definition code_rel_def:
               lookup n c2 = SOME (arity + 1, exp_opt))
 End
 
-(*
-Theorem evaluate_rewrite_tmc:
-   ∀xs ^s env1 r t opt s' acc env2 loc ts ty.
-     evaluate (xs, env1, s) = (r, t) ∧
-     env_rel ty opt acc env1 env2 ∧
-     state_rel s s' /\
-     ty_rel env1 ts ∧
-     (opt ⇒ LENGTH xs = 1) ∧
-     r ≠ Rerr (Rabort Rtype_error) ⇒
-       ?t'.
-       evaluate (xs, env2, s') = (r, t') /\
-       state_rel t t' /\
-       (opt ⇒
-         ∀op n exp arity.
-           lookup loc s.code = SOME (arity, exp) ∧
-           optimized_code loc arity exp n s'.code op ∧
-           op_type op = ty /\
-           (∃op1 tt ty r.
-             scan_expr ts loc [HD xs] = [(tt, ty, r, SOME op1)] ∧
-             ty <> Any /\ op1 <> Noop /\ op_type op1 = op_type op) ⇒
-               let (lr, x) = rewrite loc n op acc ts (HD xs) in
-                 ?rrr t1 t2.
-                 evaluate ([x], env2, s') = (rrr,t1) /\
-                 evaluate ([apply_op op (Var acc) (HD xs)],
-                   env2, s') = (rrr,t2) /\
-                 state_rel t t1 /\
-                 state_rel t t2)
+Definition optimized_code_def:
+  optimized_code loc arity exp n c =
+    ∃exp_aux exp_opt.
+        compile_exp loc n arity exp = SOME (exp_aux, exp_opt) ∧
+        lookup loc c                = SOME (arity, exp_aux) ∧
+        lookup n c                  = SOME (arity + 1, exp_opt)
+End
+
+(* Copied *)
+Definition free_names_def:
+  free_names n (name: num) ⇔ ∀k. n + bvl_to_bvi_namespaces*k ≠ name
+End
+
+(* Copied *)
+Definition namespace_rel_def:
+  namespace_rel (c1:'a spt) (c2:'a spt) ⇔
+    (∀n. n ∈ domain c2 ∧ bvl_num_stubs ≤ n ⇒ if in_ns_2 n then n ∉ domain c1 else n ∈ domain c1) ∧
+    (∀n. n ∈ domain c1 ∧ bvl_num_stubs ≤ n ⇒ ¬(in_ns_2 n)) ∧
+    (∀n. n ∈ domain c2 ∧ n < bvl_num_stubs ⇒ n ∈ domain c1)
+End
+
+(* Copied *)
+Definition input_condition_def:
+  input_condition next prog ⇔
+    EVERY (free_names next o FST) prog ∧
+   ALL_DISTINCT (MAP FST prog) ∧
+   EVERY ($~ o in_ns_2 o FST) (FILTER ((<=) bvl_num_stubs o FST) prog) ∧
+   bvl_num_stubs ≤ next ∧ in_ns_2 next
+End
+
+(* Copied *)
+Definition state_rel_def:
+  state_rel s (t:('a,'ffi) bviSem$state) ⇔
+    t.refs = s.refs ∧
+    t.clock = s.clock ∧
+    t.global = s.global ∧
+    t.ffi = s.ffi ∧
+    t.compile_oracle = state_co compile_prog s.compile_oracle ∧
+    s.compile = state_cc compile_prog t.compile ∧
+    code_rel s.code t.code ∧
+    namespace_rel s.code t.code ∧
+    (∀n. let ((next,cfg),prog) = s.compile_oracle n in
+            input_condition next prog) ∧
+    (∀n. n ∈ domain t.code ∧ in_ns_2 n ⇒ n < FST(FST(s.compile_oracle 0)))
+End
+
+Theorem compile_prog_code_rel:
+   compile_prog next prog = (next1, prog2) ∧
+   ALL_DISTINCT (MAP FST prog) ∧
+   EVERY (free_names next o FST) prog ⇒
+     code_rel (fromAList prog) (fromAList prog2)
 Proof
   cheat
 QED
-*)
 
+(* Copied *)
+(* Original with types:
+     ∀(xs :bvi$exp list) (s :(num # γ, 'ffi) state) (env1 :v list)
+         (r :(v list, v) result) (t :(num # γ, 'ffi) state) (opt :bool)
+         (s' :(γ, 'ffi) state) (acc :num) (env2 :v list) (loc :num)
+         (ts :v_ty list) (ty :v_ty).
+       evaluate (xs,env1,s) = (r,t) ∧ env_rel ty opt acc env1 env2 ∧
+       state_rel s s' ∧ ty_rel env1 ts ∧ (opt ⇒ LENGTH xs = (1 :num)) ∧
+       r ≠ (Rerr (Rabort Rtype_error :v error_result) :(v list, v) result) ⇒
+       ∃(t' :(γ, 'ffi) state).
+         evaluate (xs,env2,s') = (r,t') ∧ state_rel t t' ∧
+         (opt ⇒
+          ∀(op :assoc_op) (n :num) (exp :bvi$exp) (arity :num).
+            lookup loc s.code = SOME (arity,exp) ∧
+            optimized_code loc arity exp n s'.code op ∧ op_type op = ty ∧
+            (∃(op1 :assoc_op) (tt :v_ty list) (ty :v_ty) (r :bool).
+               scan_expr ts loc [HD xs] = [(tt,ty,r,SOME op1)] ∧ ty ≠ Any ∧
+               op1 ≠ Noop ∧ op_type op1 = op_type op) ⇒
+            (let
+               ((lr :bool),(x :bvi$exp)) = rewrite loc n op acc ts (HD xs)
+             in
+               ∃(rrr :(v list, v) result) (t1 :(γ, 'ffi) state)
+                   (t2 :(γ, 'ffi) state).
+                 evaluate ([x],env2,s') = (rrr,t1) ∧
+                 evaluate ([apply_op op (Var acc :bvi$exp) (HD xs)],env2,s') =
+                 (rrr,t2) ∧ state_rel t t1 ∧ state_rel t t2)): thm
+*)
+Theorem evaluate_rewrite_tmc:
+   ∀xs ^s env1 r t opt s' env2 loc.
+     evaluate (xs, env1, s) = (r, t) ∧
+     env_rel env1 env2 ∧
+     state_rel s s' ∧
+     (opt ⇒ LENGTH xs = 1) ∧
+     r ≠ Rerr (Rabort Rtype_error) ⇒
+       ?t'.
+       evaluate (xs, env2, s') = (r, t') ∧
+       state_rel t t' ∧
+       (opt ⇒
+         ∀n exp arity.
+           lookup loc s.code = SOME (arity, exp) ∧
+           optimized_code loc arity exp n s'.code ∧
+           (∃loc_op.
+             rewrite_aux loc loc_op arity (HD xs) = SOME aux) ⇒
+               (* let x = rewrite_opt loc arity (arity + 1) (arity + 2) (HD xs) in *)
+                 ∃rrr t1 t2.
+                   evaluate ([aux], env2, s') = (rrr,t1) ∧
+                   evaluate (xs, env2, s') = (rrr,t2) ∧
+                   state_rel t t1 ∧
+                   state_rel t t2)
+Proof
+  cheat
+QED
+
+(* Copied *)
+Theorem evaluate_compile_prog:
+   input_condition next prog ∧
+   (∀n next cfg prog. co n = ((next,cfg),prog) ⇒ input_condition next prog) ∧
+   (∀n. MEM n (MAP FST (SND (compile_prog next prog))) ∧ in_ns_2 n ⇒ n < FST (FST (co 0))) ∧
+   evaluate ([Call 0 (SOME start) [] NONE], [],
+             initial_state ffi0 (fromAList prog) co
+                 (state_cc compile_prog cc) k) = (r, s) ∧
+   r ≠ Rerr (Rabort Rtype_error) ⇒
+   ∃s2.
+     evaluate
+      ([Call 0 (SOME start) [] NONE], [],
+        initial_state ffi0 (fromAList (SND (compile_prog next prog)))
+            (state_co compile_prog co) cc k)
+      = (r, s2) ∧
+     state_rel s s2
+Proof
+  rw []
+  >> qmatch_asmsub_abbrev_tac `(es,env,st1)`
+  >> `env_rel env env` by fs [env_rel_def]
+  >> Cases_on `compile_prog next prog`
+  >> fs []
+  >> drule (GEN_ALL compile_prog_code_rel)
+  >> strip_tac
+  >> qmatch_goalsub_abbrev_tac`(es,env,st2)`
+  >> `state_rel st1 st2` by cheat
+  >> drule evaluate_rewrite_tmc
+  >> disch_then (qspec_then `F` drule)
+  cheat
+QED
+
+(* Copied *)
 Theorem compile_prog_semantics:
    input_condition n prog ∧
    (∀k n cfg prog. co k = ((n,cfg),prog) ⇒ input_condition n prog) ∧
